wip: poly1305

code/experimental/poly1305/Hacl.Impl.Poly1305.Fields.fst
@@ -1,72 +1,79 @@
 module Hacl.Impl.Poly1305.Fields
 
 module ST = FStar.HyperStack.ST
+
 open FStar.HyperStack
 open FStar.HyperStack.All
+
 open Lib.IntTypes
 open Lib.Buffer
 open Lib.ByteBuffer
+open Lib.IntVector
+
+module S = Hacl.Spec.Poly1305.Vec
+module LSeq = Lib.Sequence
+module BSeq = Lib.ByteSequence
 module F32xN = Hacl.Impl.Poly1305.Field32xN
 open F32xN
 
-type field_spec = 
-  | M32 
-  | M128 
+type field_spec =
+  | M32
+  | M128
   | M256
 
-unfold 
+unfold
 let width (s:field_spec) : lanes =
   match s with
-  | M32 -> 1
+  | M32  -> 1
   | M128 -> 2
   | M256 -> 4
-  
+
 unfold
-let limb (s:field_spec) = 
+let limb (s:field_spec) =
   match s with
-  | M32 -> F32xN.uint64xN 1
+  | M32  -> F32xN.uint64xN 1
   | M128 -> F32xN.uint64xN 2
   | M256 -> F32xN.uint64xN 4
 
 unfold
 let limb_zero (s:field_spec) : limb s=
   match s with
-  | M32 -> F32xN.zero 1 
+  | M32  -> F32xN.zero 1
   | M128 -> F32xN.zero 2
   | M256 -> F32xN.zero 4
-  
+
 unfold
 let wide (s:field_spec) =
   match s with
-  | M32 -> F32xN.uint64xN 1
+  | M32  -> F32xN.uint64xN 1
   | M128 -> F32xN.uint64xN 2
   | M256 -> F32xN.uint64xN 4
 
 unfold
 let nlimb (s:field_spec) : size_t =
   match s with
-  | M32 -> 5ul
+  | M32  -> 5ul
   | M128 -> 5ul
   | M256 -> 5ul
 
 unfold
 let blocklen (s:field_spec) : size_t =
   match s with
-  | M32 -> 16ul
+  | M32  -> 16ul
   | M128 -> 32ul
   | M256 -> 64ul
 
 unfold
 let nelem (s:field_spec) : size_t =
   match s with
-  | M32 -> 1ul
+  | M32  -> 1ul
   | M128 -> 2ul
   | M256 -> 4ul
 
 unfold
 let precomplen (s:field_spec) : size_t =
   match s with
-  | M32 -> 20ul
+  | M32  -> 20ul
   | M128 -> 20ul
   | M256 -> 20ul
 
@@ -76,190 +83,304 @@ type felem_wide (s:field_spec) = lbuffer (wide s) (nlimb s)
 type precomp_r (s:field_spec) = lbuffer (limb s) (precomplen s)
 
 noextract
-val felem_fits: (#s:field_spec) -> h:mem -> f:felem s -> m:scale32_5 -> Type0
-let felem_fits #s h f m = 
+val felem_fits: #s:field_spec -> h:mem -> f:felem s -> m:scale32_5 -> Type0
+let felem_fits #s h f m =
   match s with
-  | M32 -> felem_fits #1 h f m
-  | M128 -> felem_fits #2 h f  m
+  | M32  -> felem_fits #1 h f m
+  | M128 -> felem_fits #2 h f m
   | M256 -> felem_fits #4 h f m
 
-
-noextract 
-val feval: #s:field_spec -> h:mem -> e:felem s -> GTot (Lib.Sequence.lseq pfelem (width s))
-let feval #s h e = 
+noextract
+val as_nat: #s:field_spec -> h:mem -> e:felem s -> GTot (LSeq.lseq nat (width s))
+let as_nat #s h e =
   match s with
-  | M32 -> feval #1 h e
+  | M32  -> fas_nat #1 h e
+  | M128 -> fas_nat #2 h e
+  | M256 -> fas_nat #4 h e
+
+noextract
+val feval: #s:field_spec -> h:mem -> e:felem s -> GTot (LSeq.lseq pfelem (width s))
+let feval #s h e =
+  match s with
+  | M32  -> feval #1 h e
   | M128 -> feval #2 h e
   | M256 -> feval #4 h e
-  
+
 inline_for_extraction
-val create_felem: s:field_spec -> StackInline (felem s)
-                   (requires (fun h -> True))
-		   (ensures (fun h0 f h1 -> live h1 f /\ stack_allocated f h0 h1 (Lib.Sequence.create 5 (zero (width s)))))
-let create_felem s = 
+val create_felem:
+    s:field_spec
+  -> StackInline (felem s)
+    (requires fun h -> True)
+    (ensures  fun h0 f h1 ->
+      stack_allocated f h0 h1 (LSeq.create 5 (zero (width s))) /\
+      fas_nat h1 f == LSeq.create (width s) 0)
+let create_felem s =
   match s with
-  | M32 -> (F32xN.create_felem 1) <: felem s
+  | M32  -> (F32xN.create_felem 1) <: felem s
   | M128 -> (F32xN.create_felem 2) <: felem s
   | M256 -> (F32xN.create_felem 4) <: felem s
 
-
 inline_for_extraction
-val load_felem_le: #s:field_spec -> f:felem s -> b:lbuffer uint8 16ul -> Stack unit
-                   (requires (fun h -> live h f /\ live h b))
-		   (ensures (fun h0 _ h1 -> modifies (loc f) h0 h1))
-let load_felem_le (#s:field_spec) (f:felem s) (b:lbuffer uint8 16ul) =
+val load_felem_le:
+    #s:field_spec
+  -> f:felem s
+  -> b:lbuffer uint8 16ul
+  -> Stack unit
+    (requires fun h -> live h f /\ live h b)
+    (ensures  fun h0 _ h1 ->
+      modifies (loc f) h0 h1 /\
+      felem_fits h1 f (1, 1, 1, 1, 1) /\
+      as_nat h1 f == LSeq.create (width s) (BSeq.nat_from_bytes_le (as_seq h0 b)))
+let load_felem_le #s f b =
+  admit();
   match s with
-  | M32 -> F32xN.load_felem_le #1 f b
+  | M32  -> F32xN.load_felem_le #1 f b
   | M128 -> F32xN.load_felem_le #2 f b
   | M256 -> F32xN.load_felem_le #4 f b
 
 inline_for_extraction
-val load_felems_le: #s:field_spec -> f:felem s -> b:lbuffer uint8 (blocklen s) -> Stack unit
-                   (requires (fun h -> live h f /\ live h b))
-		   (ensures (fun h0 _ h1 -> modifies (loc f) h0 h1))
-let load_felems_le (#s:field_spec) (f:felem s) (b:lbuffer uint8 (blocklen s)) =
+val load_felems_le:
+    #s:field_spec
+  -> f:felem s
+  -> b:lbuffer uint8 (blocklen s)
+  -> Stack unit
+    (requires fun h -> live h f /\ live h b)
+    (ensures  fun h0 _ h1 ->
+      modifies (loc f) h0 h1 /\
+      felem_fits h1 f (1, 1, 1, 1, 1) /\
+      feval h1 f == S.load_elem #(width s) (as_seq h0 b))
+let load_felems_le #s f b =
+  admit();
   match s with
-  | M32 -> F32xN.load_felems_le #1 f b
+  | M32  -> F32xN.load_felems_le #1 f b
   | M128 -> F32xN.load_felems_le #2 f b
   | M256 -> F32xN.load_felems_le #4 f b
 
 inline_for_extraction
-val store_felem_le: #s:field_spec -> b:lbuffer uint8 16ul -> f:felem s -> Stack unit
-                   (requires (fun h -> live h f /\ live h b))
-		   (ensures (fun h0 _ h1 -> modifies (loc b |+| loc f) h0 h1))
-let store_felem_le #s b f = 
+val store_felem_le:
+    #s:field_spec
+  -> b:lbuffer uint8 16ul
+  -> f:felem s
+  -> Stack unit
+    (requires fun h -> live h f /\ live h b)
+    (ensures  fun h0 _ h1 -> modifies (loc b |+| loc f) h0 h1)
+let store_felem_le #s b f =
   match s with
-  | M32 -> F32xN.store_felem_le #1 b f 
-  | M128 -> F32xN.store_felem_le #2 b f 
-  | M256 -> F32xN.store_felem_le #4 b f 
+  | M32  -> F32xN.store_felem_le #1 b f
+  | M128 -> F32xN.store_felem_le #2 b f
+  | M256 -> F32xN.store_felem_le #4 b f
+
+#set-options "--z3rlimit 50"
 
 inline_for_extraction
-val set_bit: #s:field_spec -> f:felem s -> i:size_t{size_v i < 130} -> Stack unit
-                   (requires (fun h -> live h f))
-		   (ensures (fun h0 _ h1 -> modifies (loc f) h0 h1))
-let set_bit (#s:field_spec) (f:felem s) (i:size_t{size_v i < 130}) = 
+val set_bit:
+    #s:field_spec
+  -> f:felem s
+  -> i:size_t{size_v i <= 128}
+  -> Stack unit
+    (requires fun h ->
+      live h f /\
+      felem_fits h f (1, 1, 1, 1, 1) /\
+      felem_less #(width s) h f (pow2 (v i)))
+    (ensures  fun h0 _ h1 ->
+      modifies (loc f) h0 h1 /\
+      felem_fits h1 f (1, 1, 1, 1, 1) /\
+     (Math.Lemmas.pow2_le_compat 128 (v i);
+      feval h1 f == LSeq.map (pfadd (pow2 (v i))) (feval h0 f)))
+let set_bit #s f i =
   match s with
-  | M32 -> F32xN.set_bit #1 f i
+  | M32  -> F32xN.set_bit #1 f i
   | M128 -> F32xN.set_bit #2 f i
   | M256 -> F32xN.set_bit #4 f i
-  
+
 inline_for_extraction
-val set_bit128: #s:field_spec -> f:felem s -> Stack unit
-                   (requires (fun h -> live h f))
-		   (ensures (fun h0 _ h1 -> modifies (loc f) h0 h1))
-let set_bit128 (#s:field_spec) (f:felem s) = 
+val set_bit128:
+    #s:field_spec
+  -> f:felem s
+  -> Stack unit
+    (requires fun h ->
+      live h f /\
+      felem_fits h f (1, 1, 1, 1, 1) /\
+      felem_less #(width s) h f (pow2 128))
+    (ensures  fun h0 _ h1 ->
+      modifies (loc f) h0 h1 /\
+      felem_fits h1 f (1, 1, 1, 1, 1) /\
+      feval h1 f == LSeq.map (pfadd (pow2 128)) (feval h0 f))
+let set_bit128 #s f =
   match s with
-  | M32 -> F32xN.set_bit128 #1 f
+  | M32  -> F32xN.set_bit128 #1 f
   | M128 -> F32xN.set_bit128 #2 f
   | M256 -> F32xN.set_bit128 #4 f
 
-
 inline_for_extraction
-val set_zero: #s:field_spec -> f:felem s -> Stack unit
-                   (requires (fun h -> live h f))
-		   (ensures (fun h0 _ h1 -> modifies (loc f) h0 h1))
-let set_zero (#s:field_spec) (f:felem s) = 
+val set_zero:
+    #s:field_spec
+  -> f:felem s
+  -> Stack unit
+    (requires fun h -> live h f)
+    (ensures  fun h0 _ h1 ->
+      modifies (loc f) h0 h1 /\
+      fas_nat h1 f == LSeq.create (width s) 0)
+let set_zero #s f =
   match s with
-  | M32 -> F32xN.set_zero #1 f
+  | M32  -> F32xN.set_zero #1 f
   | M128 -> F32xN.set_zero #2 f
   | M256 -> F32xN.set_zero #4 f
 
 inline_for_extraction
-val copy_felem: #s:field_spec -> f:felem s -> f':felem s -> Stack unit
-                   (requires (fun h -> live h f /\ live h f'))
-		   (ensures (fun h0 _ h1 -> modifies (loc f) h0 h1))
-let copy_felem (#s:field_spec) (f:felem s) (f':felem s) = 
+val copy_felem:
+    #s:field_spec
+  -> f:felem s
+  -> f':felem s
+  -> Stack unit
+    (requires fun h ->
+      live h f /\ live h f' /\ disjoint f f')
+    (ensures  fun h0 _ h1 ->
+      modifies (loc f) h0 h1 /\
+      fas_nat #(width s) h1 f == fas_nat h0 f')
+let copy_felem #s f f' =
   match s with
-  | M32 -> F32xN.copy_felem #1 f f'
+  | M32  -> F32xN.copy_felem #1 f f'
   | M128 -> F32xN.copy_felem #2 f f'
   | M256 -> F32xN.copy_felem #4 f f'
 
-
 inline_for_extraction
-val reduce_felem: #s:field_spec -> f:felem s -> Stack unit
-                   (requires (fun h -> live h f))
-		   (ensures (fun h0 _ h1 -> modifies (loc f) h0 h1))
-let reduce_felem #s f =
+val reduce_felem:
+    #s:field_spec
+  -> f:felem s
+  -> Stack unit
+    (requires fun h ->
+      live h f /\ acc_inv_t (as_tup5 #(width s) h f))
+    (ensures  fun h0 _ h1 ->
+      modifies (loc f) h0 h1 /\
+      feval h1 f == feval h0 f /\
+      felem_less #(width s) h1 f prime)
+let reduce_felem #s f = admit();
   match s with
-  | M32 -> F32xN.reduce_felem #1 f
+  | M32  -> F32xN.reduce_felem #1 f
   | M128 -> F32xN.reduce_felem #2 f
   | M256 -> F32xN.reduce_felem #4 f
-  
+
 inline_for_extraction
-val load_precompute_r: #s:field_spec -> p:precomp_r s -> r0:uint64 -> r1:uint64 -> Stack unit
-                   (requires (fun h -> live h p))
-		   (ensures (fun h0 _ h1 -> modifies (loc p) h0 h1 ))
-let load_precompute_r #s p r0 r1 = 
+val load_precompute_r:
+    #s:field_spec
+  -> p:precomp_r s
+  -> r0:uint64
+  -> r1:uint64
+  -> Stack unit
+    (requires fun h -> live h p)
+    (ensures  fun h0 _ h1 -> modifies (loc p) h0 h1)
+let load_precompute_r #s p r0 r1 =
   match s with
-  | M32 -> F32xN.load_precompute_r #1 p r0 r1
+  | M32  -> F32xN.load_precompute_r #1 p r0 r1
   | M128 -> F32xN.load_precompute_r #2 p r0 r1
   | M256 -> F32xN.load_precompute_r #4 p r0 r1
 
-
 inline_for_extraction
-val fadd_mul_r: #s:field_spec -> out:felem s -> f1:felem s -> precomp:precomp_r s -> Stack unit
-                   (requires (fun h -> live h out /\ live h f1 /\ live h precomp))
-		   (ensures (fun h0 _ h1 -> modifies (loc out) h0 h1))
+val fadd_mul_r:
+    #s:field_spec
+  -> out:felem s
+  -> f1:felem s
+  -> precomp:precomp_r s
+  -> Stack unit
+    (requires fun h ->
+      live h out /\ live h f1 /\ live h precomp /\
+     (let r = gsub precomp 0ul 5ul in
+      let r_5 = gsub precomp 5ul 5ul in
+      felem_fits h out (1, 2, 1, 1, 1) /\
+      felem_fits h f1 (1, 1, 1, 1, 1) /\
+      felem_fits h r (1, 1, 1, 1, 1) /\
+      felem_fits h r_5 (5, 5, 5, 5, 5) /\
+      as_tup5 #(width s) h r_5 == precomp_r5 (as_tup5 h r)))
+    (ensures  fun h0 _ h1 ->
+      modifies (loc out) h0 h1 /\
+     (let r = gsub precomp 0ul 5ul in
+      acc_inv_t #(width s) (as_tup5 h1 out) /\
+      feval h1 out == LSeq.map2 (pfmul) (LSeq.map2 (pfadd) (feval h0 out) (feval h0 f1)) (feval h0 r)))
 let fadd_mul_r #s out f1 precomp =
   match s with
-  | M32 -> F32xN.fadd_mul_r #1 out f1 precomp
+  | M32  -> F32xN.fadd_mul_r #1 out f1 precomp
   | M128 -> F32xN.fadd_mul_r #2 out f1 precomp
   | M256 -> F32xN.fadd_mul_r #4 out f1 precomp
 
 inline_for_extraction
-val fmul_rn: #s:field_spec -> out:felem s -> f1:felem s -> precomp:precomp_r s -> Stack unit
-                   (requires (fun h -> live h out /\ live h f1 /\ live h precomp /\
-				    (let rn = gsub precomp 10ul 5ul in
-				     let rn_5 = gsub precomp 15ul 5ul in
-				     felem_fits h out (2,3,2,2,2) /\
-				     felem_fits h rn (1,2,1,1,1) /\
-				     felem_fits h rn_5 (5,10,5,5,5) /\
-				     as_tup5 #(width s) h rn_5 == precomp_r5 (as_tup5 h rn))))
-		   (ensures (fun h0 _ h1 -> modifies (loc out) h0 h1 /\ 
-					 (let rn = gsub precomp 10ul 5ul in 
-					  acc_inv_t #(width s) (as_tup5 h1 out) /\
-					  feval h1 out == Lib.Sequence.map2 pfmul (feval h0 f1) (feval h0 rn))))
+val fmul_rn:
+    #s:field_spec
+  -> out:felem s
+  -> f1:felem s
+  -> precomp:precomp_r s
+  -> Stack unit
+    (requires fun h ->
+      live h out /\ live h f1 /\ live h precomp /\
+     (let rn = gsub precomp 10ul 5ul in
+      let rn_5 = gsub precomp 15ul 5ul in
+      felem_fits h out (2,3,2,2,2) /\
+      felem_fits h rn (1,2,1,1,1) /\
+      felem_fits h rn_5 (5,10,5,5,5) /\
+      as_tup5 #(width s) h rn_5 == precomp_r5 (as_tup5 h rn)))
+    (ensures fun h0 _ h1 ->
+      modifies (loc out) h0 h1 /\
+     (let rn = gsub precomp 10ul 5ul in
+      acc_inv_t #(width s) (as_tup5 h1 out) /\
+      feval h1 out == LSeq.map2 pfmul (feval h0 f1) (feval h0 rn)))
 let fmul_rn #s out f1 precomp =
   admit();
   match s with
-  | M32 -> F32xN.fmul_rn #1 out f1 precomp
+  | M32  -> F32xN.fmul_rn #1 out f1 precomp
   | M128 -> F32xN.fmul_rn #2 out f1 precomp
   | M256 -> F32xN.fmul_rn #4 out f1 precomp
 
-let norm (#w:lanes) (n:Lib.Sequence.lseq pfelem w) (r:pfelem) = 
+let norm (#w:lanes) (n:LSeq.lseq pfelem w) (r:pfelem) =
   match w with
   | 1 -> pfmul n.[0] r
   | 2 -> let r2 = pfmul r r in pfadd (pfmul n.[0] r2) (pfmul n.[1] r)
-  | 4 -> let r2 = pfmul r r in let r3 = pfmul r2 r in let r4 = pfmul r2 r2 in 
+  | 4 -> let r2 = pfmul r r in let r3 = pfmul r2 r in let r4 = pfmul r2 r2 in
 	pfadd (pfmul n.[0] r4) (pfadd (pfmul n.[1] r3) (pfadd (pfmul n.[2] r2) (pfmul n.[3] r)))
 
 
 inline_for_extraction
-val fmul_rn_normalize: #s:field_spec -> out:felem s -> precomp:precomp_r s -> Stack unit
-                   (requires (fun h -> live h out /\ live h precomp /\
-				    (let r = gsub precomp 0ul 5ul in
-				     let r_5 = gsub precomp 5ul 5ul in
-				     felem_fits h out (2,3,2,2,2) /\
-				     felem_fits h r (1,1,1,1,1) /\
-				     felem_fits h r_5 (5,5,5,5,5) /\
-				     as_tup5 #(width s) h r_5 == precomp_r5 (as_tup5 h r))))
-		   (ensures (fun h0 _ h1 -> modifies (loc out |+| loc precomp) h0 h1 /\ 
-					 (let r = (feval h0 (gsub precomp 0ul 5ul)).[0] in 
-					  acc_inv_t #(width s) (as_tup5 h1 out) /\
-					  (feval h1 out).[0] == norm (feval h0 out) r)))
+val fmul_rn_normalize:
+    #s:field_spec
+  -> out:felem s
+  -> precomp:precomp_r s
+  -> Stack unit
+    (requires fun h ->
+      live h out /\ live h precomp /\
+     (let r = gsub precomp 0ul 5ul in
+      let r_5 = gsub precomp 5ul 5ul in
+      felem_fits h out (2,3,2,2,2) /\
+      felem_fits h r (1,1,1,1,1) /\
+      felem_fits h r_5 (5,5,5,5,5) /\
+      as_tup5 #(width s) h r_5 == precomp_r5 (as_tup5 h r)))
+    (ensures fun h0 _ h1 ->
+      modifies (loc out |+| loc precomp) h0 h1 /\
+     (let r = (feval h0 (gsub precomp 0ul 5ul)).[0] in
+      acc_inv_t #(width s) (as_tup5 h1 out) /\
+     (feval h1 out).[0] == norm (feval h0 out) r))
 let fmul_rn_normalize #s out precomp =
   admit();
   match s with
-  | M32 -> F32xN.fmul_rn_normalize #1 out precomp
+  | M32  -> F32xN.fmul_rn_normalize #1 out precomp
   | M128 -> F32xN.fmul_rn_normalize #2 out precomp
   | M256 -> F32xN.fmul_rn_normalize #4 out precomp
- 
+
 inline_for_extraction
-val fadd: #s:field_spec -> out:felem s -> f1:felem s -> f2:felem s -> Stack unit
-                   (requires (fun h -> live h out /\ live h f1 /\ live h f2 /\ felem_fits h f1 (1,2,1,1,1) /\ felem_fits h f2 (1,1,1,1,1)))
-		   (ensures (fun h0 _ h1 -> modifies (loc out) h0 h1 /\ felem_fits h1 out (2,3,2,2,2) /\ feval h1 out == Lib.Sequence.map2 pfadd (feval h0 f1) (feval h0 f2)))
-let fadd #s out f1 f2=
+val fadd:
+    #s:field_spec
+  -> out:felem s
+  -> f1:felem s
+  -> f2:felem s
+  -> Stack unit
+    (requires fun h ->
+      live h out /\ live h f1 /\ live h f2 /\
+      felem_fits h f1 (1,2,1,1,1) /\
+      felem_fits h f2 (1,1,1,1,1))
+    (ensures fun h0 _ h1 ->
+      modifies (loc out) h0 h1 /\
+      felem_fits h1 out (2,3,2,2,2) /\
+      feval h1 out == LSeq.map2 pfadd (feval h0 f1) (feval h0 f2))
+let fadd #s out f1 f2 =
   match s with
-  | M32 -> F32xN.fadd #1 out f1 f2 
-  | M128 -> F32xN.fadd #2 out f1 f2 
-  | M256 -> F32xN.fadd #4 out f1 f2 
+  | M32  -> F32xN.fadd #1 out f1 f2
+  | M128 -> F32xN.fadd #2 out f1 f2
+  | M256 -> F32xN.fadd #4 out f1 f2
